# Kernelize SVM
- Till now we have directly used $\phi(x_n)$ and formulated SVM based on it
- We will kernelize SVM by solving its dual problem which is easily kernelizable
- We will show that the dual problem gives the same solution as the original problem
$\newcommand{\pd}[2]{\frac{\partial{#1}}{\partial{#2}}}$
**Lagrangian**
$$L(x,\alpha,\beta) = f_0(x) + \sum^m_{i=1}\alpha_i f_i(x) + \sum^p_{j=1}\beta_jh_j(x)$$
$\alpha, \beta$ = Lagrange multiplier

**Deriving the dual form**
Primal SVM: $\underset{w,b,s}{min} \frac {1}{2} ||w||^2_2 + C \sum_n s_n$ s.t. $1-s_n-y_n[w^T\phi(x_n)+b]\leq0$, $n \in 1,\dots,N$ $-s_n \leq 0$ 
Lagrangian
$$
\begin{align}
&L(w,b,\{s_n\},\{\alpha_n\},\{\lambda_n\}) \\
&= C\sum_n s_n + \frac {1}{2} ||w||^2_2 + \sum_n \alpha_n\{1-y_n[w^T\phi(x_n)+b]-s_n\}-\sum_n\lambda_n s_n
\end{align}
$$
The dual problem
Primal: $\underset{w,b,s_i}{min} \underset{\alpha , \lambda,\\ \alpha \geq 0 \lambda \geq 0}{max} L(w,b,s,\alpha, \lambda)$ 
Dual:$\underset{\alpha , \lambda,\\ \alpha \geq 0 \lambda \geq 0}{max} \underset{w,b,s_i}{min}  L(w,b,s,\alpha, \lambda)$

**Goal**: Solve for $\underset{w,b,s}{min} L(w,b,s,\alpha, \lambda) \rightarrow g(\alpha, \lambda)$ 
Necessary (and sufficient) condition for optimality $\rightarrow$ $\nabla_w L = 0, \nabla_b L = 0, \nabla_s L = 0$ 

$\nabla_w L = w - \sum_n y_n\alpha_n \phi(x_n) = 0$  ($\pd {||w||^2} w = 2w$, $\pd w w = 1$ )
$\nabla_b L = \sum \alpha_n y_n = 0$
$\nabla_s L = C -\alpha_n -\lambda_n = 0$
From this we obtain,
$w =\sum_n y_n\alpha_n \phi(x_n)$ | $\lambda_n = C-\alpha_n$ 

Plugging the parameters, we obtain the Dual that does not depend on $\lambda$
$$\underset{\alpha}{max} \sum_n \alpha_n -\frac{1}{2} \sum_{m,n} y_my_n \alpha_m \alpha_n \phi(x_m) \phi(x_n)$$
**Complementary slackness (KKT)**
The product of lagrange multiplier and the value of the primal equals zero
$\begin{cases} \lambda_n s_n = 0 \\ \alpha_n \{1-s_n - y_n[w^T\phi(x_n)+b]\} = 0\end{cases}$
Implication: 
If $\lambda_n >0$, then $s_n$ = 0. $\lambda = C-\alpha_n$ $\rightarrow$ if $\lambda_n =0$ then $\alpha_n = C$ 
If $\alpha_n >0$ i.e. $x_n$ plays a role in the solution $\rightarrow$ $1-s_n -y_n[w^T\phi(x_n)+b] = 0$ 
								Or   $y_n[w^T\phi(x_n)+b] = 1-s_n$
Three things can happen
- If $s_n = 0$ then $y_n[w^T\phi(x_n)+b] =1$
- If $s_n >0$ and $s_n \in (0,1)$, then $y_n[w^T\phi(x_n)+b] = 1-s_n >0$
- If $s_n>1$, then $y_n[w^T\phi(x_n)+b] <0$ 



